secure_api/merkle_tree/MerkleTree.New.Low.Datastructures.fst
@@ -315,4 +315,3 @@ val hash_vv_as_seq_get_index:
 #push-options "--z3rlimit 20"
 let hash_vv_as_seq_get_index #_ h hvv i j = ()
 #pop-options
-
